results after session with Son Ho, proof for N=1 is almost finished

test/lean/Proofs.lean
@@ -9,30 +9,69 @@ namespace test
 
 namespace arithmetics
 
-def BigInt.valImpl [Inhabited U64] (l : List U64) : Int :=
-  if l.len = 0
-  then 0
-  else (l.index 0) + (valImpl (l.idrop 1)) * (2 ^ 64)
-termination_by BigInt.valImpl l => l.len.toNat
-decreasing_by
-  simp_wf
-  have : 1 ≤ l.len := by scalar_tac
-  simp [Int.toNat_sub_of_le, *]
-  sorry
+def BigInt.valImpl (l : List U64) : Int :=
+  match l with
+  | a::b => a.val + (valImpl b) * (2 ^ 64)
+  | [] => 0
+
+@[simp]
+lemma tmp : Inhabited U64 := by
+  constructor
+  apply 0#u64
+
+-- Biggest part by Son Ho
+lemma BigInt.update_eq [Inhabited U64] (l : List U64) (i : Int) (x : U64)
+  (h0 : 0 ≤ i) (h1 : i < l.len) :
+  BigInt.valImpl (l.update i x) = BigInt.valImpl l + (x - l.index i) * ((2 ^ 64) ^ i.toNat) := by
+  match l with
+  | [] =>
+    -- Contradiction: 0 ≤ i ∧ i < 0
+    simp at h1
+    scalar_tac
+  | h :: tl =>
+    simp at *
+    if i = 0 then
+      simp [*] -- By writing [*] I'm using the hypothesis i = 0
+      unfold valImpl
+      scalar_tac
+    else
+      have hnz : i ≠ 0 := by scalar_tac
+      -- This uses update_nzero_cons and index_nzero_cons
+      simp [*] -- By writing [*] I'm using the hypothesis i ≠ 0
+      unfold valImpl
+      -- Recursive call
+      have heq := update_eq tl (i - 1) x (by scalar_tac) (by scalar_tac)
+      rw [heq]
+      rw [add_mul]
+      simp []
+      have hexpr (y : Int) : y * (2 ^ 64) ^ (Int.toNat i - 1) * 2 ^ 64 = y * (2 ^ 64) ^ Int.toNat i := by {
+        rw [←pow_mul]
+        rw [mul_assoc]
+        simp []
+        rw [←pow_add]
+        rw [←pow_mul]
+        rw [Nat.mul_sub_left_distrib]
+        rw [←Nat.sub_add_comm]
+        simp [*]
+        have hgone : i ≥ 1 := by scalar_tac
+        simp [hgone, *]
+      }
+      rw [hexpr]
+      simp [add_assoc]
 
 
--- def BigInt.valImpl (l : List U64) : Int :=
---   match l with
---   | a::b => a.val + (valImpl b) * (2 ^ 64)
---   | [] => 0
+lemma BigInt.len_spec
+  (N : Usize) (self : arithmetics.BigInt N) :
+  self.num.val.len = N.val := by
+  have h := self.num.property
+  rw [List.len_eq_length]
+  apply h
 
 def BigInt.val {N : Usize} [Inhabited U64] (x : BigInt N) : Int := valImpl x.num.val
 
-def BigInt.max_value [Inhabited U64] (N : Usize) : Int := (U64.max + 1) ^ (Int.toNat N.val) - 1
+def BigInt.mod_value (N : Usize) : Int := (U64.max + 1) ^ (Int.toNat N.val)
 
-lemma tmp: 
-  ∀ (N : Usize) (self : arithmetics.BigInt N),
-  self.num.val.len = N.val := by intro N; intro self; simp [List.len_eq_length]; sorry
+def BigInt.max_value (N : Usize) : Int := BigInt.mod_value N - 1
 
 theorem adc_for_add_with_carry_spec (a : U64) (b : U64) (carry : U8) :
   ∃ new_carry, adc_for_add_with_carry a b carry = .ret new_carry ∧ 
@@ -49,10 +88,11 @@ lemma add_with_carry_overflow [Inhabited U64] :
   ¬b ↔ self.val + other.val ≤ BigInt.max_value N := sorry
     -- by unfold arithmetics.BigInt.add_with_carry
 
+-- Biggest part by Son Ho
 lemma add_with_carry_correct [Inhabited U64] :
   ∀ (N : Usize) (self : arithmetics.BigInt N) (other : arithmetics.BigInt N),
   ∃ v, arithmetics.BigInt.add_with_carry_back N self other = .ret v ∧
-  v.val = (self.val + other.val) % (BigInt.max_value N) := by
+  v.val = (self.val + other.val) % (BigInt.mod_value N) := by
     simp [arithmetics.BigInt.add_with_carry_back]
     intro N
     if hx : N = 1#usize then
@@ -64,15 +104,30 @@ lemma add_with_carry_correct [Inhabited U64] :
       progress with adc_for_add_with_carry_back_spec as ⟨ i1, hi1 ⟩
       progress with Array.update_usize_spec as ⟨ a1, ha1 ⟩
       simp [BigInt.val, BigInt.max_value]
-      have h_self_val : i = self.val := by simp [hi, BigInt.val]; unfold BigInt.valImpl; simp [tmp, *]; unfold BigInt.valImpl; simp [tmp, *];
-      have h_bi_1_val : ∀ (bi : arithmetics.BigInt 1#usize), BigInt.valImpl bi.num.val = (bi.num.val).index 0#usize.val  := by intros; simp [hi, BigInt.val]; unfold BigInt.valImpl; simp [tmp, *]; unfold BigInt.valImpl; simp [tmp, *];
+      -- have h_self_val : i = self.val := by simp [hi, BigInt.val]; unfold BigInt.valImpl; simp [tmp, *]; unfold BigInt.valImpl; simp [tmp, *];
+      have h_bi_1_val : ∀ (bi : arithmetics.BigInt 1#usize), BigInt.valImpl bi.num.val = (bi.num.val).index 0#usize.val  := by intros; simp [hi, BigInt.val]; unfold BigInt.valImpl; sorry
+      -- Proving that a1.val.len = 1 (remark: scalar_tac does it automatically)
+      -- have h_array := a1.property
+      have h_valImpl := BigInt.update_eq self.num.val 0 i1 (by simp) (by scalar_tac)
       simp [h_bi_1_val]
       simp [ha1]
-      unfold BigInt.valImpl
-      simp []
+      rw [h_valImpl]
+      simp
+      -- Because length = 1
+      have hself : BigInt.valImpl self.num.val = (self.num.val.index 0).val := by unfold BigInt.valImpl; sorry
+      rw [hself]
+      
+      rw [hi1]
+      
+      have h64 : BigInt.mod_value 1#usize = 2 ^ 64 := by unfold BigInt.mod_value; simp []
+      rw [h64]
+      -- Finishing the proof
+      rw [hi0]
+      simp
+      rw [hi]
+      simp
+    else
       sorry
-    else 
-    sorry
 
 end arithmetics
 
